tests/lean/run/smt_tests.lean
@@ -4,8 +4,6 @@ constant p    : nat → nat → Prop
 constants a b : nat
 constant h    : p (a + 1 * b + 0) (a + b)
 
-set_option trace.app_builder true
-
 open tactic smt_tactic
 
 def ex : p (a + b) (a + b) :=
@@ -17,4 +15,34 @@ begin [smt]
     new_h ← mk_app `eq.mp [he, h],
     exact new_h
   }
+end
+
+def foo : nat → nat
+| 0     := 0
+| (n+1) := 2*n
+
+example (n : nat) : n = 0 → foo (n+1) = 2*0 :=
+begin [smt]
+  add_lemma [mul_zero, zero_mul],
+  add_eqn_lemmas foo,
+  ematch
+end
+
+example (n : nat) : n = 0 → foo n = 0 :=
+begin [smt]
+  add_eqn_lemmas foo
+end
+
+def boo : nat → nat
+| 0     := 1
+| (n+1) :=
+  match foo n with
+  | 0 := 2
+  | _ := 3
+  end
+
+example (n : nat) : n = 0 → boo (n+1) = 2 :=
+begin [smt]
+  add_eqn_lemmas boo foo,
+  ematch,
 end
